first working version in lean3

kruskal.lean
@@ -1,5 +1,5 @@
-import data.list tools.super
-open nat function
+import data.list tools.super .library_dev.data.list.comb .library_dev.data.list.set 
+open nat function tactic
 
 -- lemmas of list
 
@@ -10,54 +10,25 @@ variables {A B: Type}
 private theorem mem_cons (x : A) (l : list A) : x ∈ x :: l :=
 or.inl rfl
 
-def upto : ℕ → list ℕ
-| 0      := []
-| (succ n) := n :: upto n
+-- def upto : ℕ → list ℕ
+-- | 0      := []
+-- | (succ n) := n :: upto n
 
-theorem lt_of_mem_upto {n i : nat} : i ∈ upto n → i < n :=
-nat.rec_on n (λ h, absurd h (not_mem_nil i)) 
-(λ a ih h, or.elim h 
-(begin intro l, rw l, apply lt_succ_self end) 
-(λ r, lt_trans (ih r) (lt_succ_self a)))
+-- theorem lt_of_mem_upto {n i : nat} : i ∈ upto n → i < n :=
+-- nat.rec_on n (λ h, absurd h (not_mem_nil i)) 
+-- (λ a ih h, or.elim h 
+-- (begin intro l, rw l, apply lt_succ_self end) 
+-- (λ r, lt_trans (ih r) (lt_succ_self a)))
 
-theorem upto_succ (n : nat) : upto (succ n) = n :: upto n := rfl
+-- theorem upto_succ (n : nat) : upto (succ n) = n :: upto n := rfl
 
-theorem length_upto : ∀ n, length (upto n) = n
-| 0        := rfl
-| (succ n) := begin simp [upto_succ, length_cons, length_upto] end
+-- theorem length_upto : ∀ n, length (upto n) = n
+-- | 0        := rfl
+-- | (succ n) := begin simp [upto_succ, length_cons, length_upto] end
 
-#print filter
-
-def dmap (p : A → Prop) [h : decidable_pred p] (f : Π a, p a → B) : list A → list B
-| [] := []
-| (a::l) := if P : (p a) then list.cons (f a P) (dmap l) else (dmap l)
 
 /- map -/
 theorem map_nil (f : A → B) : list.map f [] = [] := rfl
-
-  section dmap
-
-  variable {p : A → Prop}
-  variable [h : decidable_pred p]
-  include h
-  variable {f : Π a, p a → B}
-
-  lemma dmap_nil : dmap p f [] = [] := rfl
-
-  lemma dmap_cons_of_pos {a : A} (P : p a) : ∀ l, dmap p f (a::l) = (f a P) :: dmap p f l :=
-  λ l, dif_pos P
-
-  lemma map_dmap_of_inv_of_pos {g : B → A} (Pinv : ∀ a (Pa : p a), g (f a Pa) = a) :
-  ∀ {l : list A}, (∀ {{ a }}, a ∈ l → p a ) → map g (dmap p f l) = l
-
-  | []     := assume Pl, by rewrite [dmap_nil, map_nil]
-  | (a::l) := assume Pal, 
-              have Pa : p a, from Pal (mem_cons _ _),
-              have Pl : ∀ a, a ∈ l → p a,
-                from take x Pxin, Pal (mem_cons_of_mem a Pxin), 
-              by rewrite [dmap_cons_of_pos Pa, map_cons, Pinv, map_dmap_of_inv_of_pos Pl]
-
-  end dmap
 
 end list
 
@@ -92,41 +63,95 @@ begin
   apply eq.symm (length_upto _)
 end 
 
+lemma mem_upto (n : nat) : ∀ (i : fin n), i ∈ upto n :=
+take i, fin.rec_on i
+  (take ival Piltn,
+    have ival ∈ list.upto n, from mem_upto_of_lt Piltn,
+mem_dmap Piltn this)
+
 end fin
 
 -- lemmas of bigops
 
-namespace group_bigops
+-- namespace group_bigops
 
-variables {A B : Type}
+-- variables {A B : Type}
 
-definition addf {A B : Type} [sgB : add_semigroup B] (f : A → B) : B → A → B :=
-λ b a, b + f a
+-- definition Suml (f : A → ℕ) : list A → ℕ 
+-- | [] := 0
+-- | (a :: ls) := f a + Suml ls
 
-definition Suml [add_monoid B] (l : list A) (f : A → B) : B :=
-list.foldl (addf f) 0 l
+-- definition addf {A B : Type} [sgB : add_semigroup B] (f : A → B) : B → A → B :=
+-- λ b a, b + f a
 
--- check add_monoid
+-- definition Suml [add_monoid B] (l : list A) (f : A → B) : B :=
+-- list.foldl (addf f) 0 l
 
-end group_bigops
+-- theorem Suml_nil (f : A → B) : Suml [] f = 0 := Prodl_nil f
+
+-- -- check add_monoid
+
+-- end group_bigops
 
 -- definitions
 
-open group_bigops list fin
+section 
+
+-- Suml
+
+variables {A : Type}
+
+definition Suml (f : A → ℕ) : list A → ℕ 
+| [] := 0
+| (a :: ls) := f a + Suml ls
+
+theorem le_add_of_le {a b c : ℕ} : a ≤ b → a ≤ b + c :=
+begin
+induction c with n ih, intro,super, intro h2,
+apply le_succ_of_le, exact ih h2
+end
+
+theorem le_of_mem_Suml {f : A → ℕ} {a : A} {l : list A} : 
+a ∈ l → f a ≤ Suml f l :=
+begin 
+induction l with b ls ih, intro h, exact absurd h (not_mem_nil _),
+dsimp [Suml], intro h, assert h' : a = b ∨ a ∈ ls, exact h,
+cases h' with l r, rw l, apply le_add_right,
+rw add_comm,apply le_add_of_le, exact ih r
+end
+
+
+end
+
+open list fin
 
 inductive finite_tree : Type
 | cons : Π {n : ℕ},  (fin n → finite_tree) → finite_tree
 
+
+
+
 namespace finite_tree
 
-definition size : finite_tree → ℕ
-| (@cons n ts) := Suml (fin.upto n) (λ i, size (ts i)) + 1
+-- definition size : finite_tree → ℕ
+-- | (@cons n ts) := Suml (fin.upto n) (λ i, size (ts i)) + 1
+def size : finite_tree → ℕ
+| (@cons n ts) := Suml (λ i, size (ts i)) (fin.upto n) + 1
 
-theorem exists_eq_cons_of_ne_nil {A : Type} {l : list A} : l ≠ [] → ∃ a, ∃ l', l = a::l' := 
-list.rec_on l (λ H, absurd rfl H) (λ a l' IH H, ⟨a, ⟨l',rfl⟩⟩)
+-- theorem exists_eq_cons_of_ne_nil {A : Type} {l : list A} : l ≠ [] → ∃ a, ∃ l', l = a::l' := 
+-- list.rec_on l (λ H, absurd rfl H) (λ a l' IH H, ⟨a, ⟨l',rfl⟩⟩)
 
 theorem pos_of_size (t : finite_tree) : 0 < size t :=
 finite_tree.rec_on t (λ n ts ih, dec_trivial)
+
+section
+parameter ts : fin 0 → finite_tree
+parameter f : ℕ → ℕ
+
+-- #eval fin.upto 0
+-- #eval Suml id []
+
+end
 
 -- theorem pos_of_Suml {n : ℕ} (H : n ≠ 0) (ts : fin n → finite_tree) : 0 < Suml (upto n) (λ i, size (ts i)) :=
 -- have upto n ≠ nil, from upto_ne_nil_of_ne_zero n H,
@@ -138,6 +163,15 @@ finite_tree.rec_on t (λ n ts ih, dec_trivial)
 -- have f a > 0, from pos_of_size (ts a),
 -- have f a + Suml l' f > 0, from add_pos_left this (Suml l' f),
 -- by+ simp
+
+theorem lt_of_size_branches_aux {n : ℕ} (ts : fin n → finite_tree) (k : fin n) : size (ts k) < Suml (λ i, size (ts i)) (upto n) + 1 := 
+begin
+assert kin : k ∈ upto n, exact mem_upto n k,
+assert h : size (ts k) ≤ Suml (λ i, size (ts i)) (upto n), 
+apply le_of_mem_Suml kin,
+apply lt_succ_of_le, assumption
+end
+
 
 -- theorem le_of_elt_Suml {n : ℕ} (ts : fin n → finite_tree) (k : fin n) : size (ts k) ≤ Suml (upto n) (λ i, size (ts i)) := -- what if n = 0?
 -- have k ∈ upto n, from mem_upto n k,
@@ -152,126 +186,99 @@ finite_tree.rec_on t (λ n ts ih, dec_trivial)
 -- have size (ts k) ≤ Suml s (λ i, size (ts i)) + Suml (k::t) (λ i, size (ts i)), from le.trans le1 this,
 -- by+ simp
 
-definition embeds : finite_tree → finite_tree → Prop
-| (@cons 0 _) _              := true
-| (@cons _ ts) (@cons 0 _)      := false
+
+def embeds : finite_tree → finite_tree → Prop
 | (@cons _ ts) (@cons _ us) := (∃ j, embeds (cons ts) (us j)) ∨
                                   (∃ f, injective f ∧ ∀ i, embeds (ts i) (us (f i)))
-
-/-
-  -- here is a "hands on" definition of the same predicate:
-  definition embeds (s t : finite_tree) : Prop :=
-  (finite_tree.rec
-    (finite_tree.rec true (λ m ss embss, false))
-    (λ n ts embts,
-      finite_tree.rec true (λ m ss embss,
-        (∃ j, embts j (cons ss)) ∨ (∃ f, injective f ∧ ∀ i, embts (f i) (ss i)))))
-  t s
--/
 
 infix ` ≼ `:50 := embeds  -- \preceq
 
 def node {ts : fin 0 → finite_tree} : finite_tree := @cons 0 ts
 
+def {u} fin_zero_absurd {α : Sort u} (i : fin 0) : α :=
+absurd i.2 (not_lt_zero i.1)
+
 theorem node_embeds {ts : fin 0 → finite_tree} (t : finite_tree) : @cons 0 ts ≼ t :=
 begin 
-  cases t with n a, cases n,
-  trivial, trivial
+  induction t with n a ih,
+  dsimp [embeds],  
+  pose f : fin 0 → fin n := λ i : fin 0, fin_zero_absurd i,
+  apply or.inr,
+  existsi f,
+  split,
+    intros i j hij, exact fin_zero_absurd i,
+  intro i, exact fin_zero_absurd i
 end
 
-theorem not_cons_embeds_node {n : ℕ} {tt : fin 0 → finite_tree} (ts : fin (succ n) → finite_tree) : ¬ cons ts ≼ @node tt :=
-λ h, begin cases n, exact h, exact h end
-
-theorem not_embeds_empty {ts : fin 0 → finite_tree} (i : fin 0) (t : finite_tree) : ¬ t ≼ ts i :=
-λ h, have i.val < 0, from i.is_lt, absurd this (not_lt_zero _)
-
--- curiously, with either definition above, this doesn't work with = and rfl
--- proposition cons_embeds_cons_iff {m n : ℕ} (ss : fin m → finite_tree) (ts : fin n → finite_tree) :
---   cons ss ≼ cons ts ↔ (∃ j, cons ss ≼ ts j) ∨ (∃ f, injective f ∧ ∀ i, ss i ≼ ts (f i)) :=
--- !iff.refl
+theorem not_embeds_node {n : ℕ} {ts : fin (succ n) → finite_tree} 
+  {tt : fin 0 → finite_tree}: ¬ cons ts ≼ cons tt := 
+begin 
+  intro h,
+  dsimp [embeds] at h,
+  cases h with h₁ h₂,
+  { cases h₁ with i hi, exact fin_zero_absurd i },  
+  cases h₂ with f hf, exact fin_zero_absurd (f ⟨0, zero_lt_succ _⟩)
+end
 
 theorem cons_embeds_cons_left {m n : ℕ} {ss : fin m → finite_tree} {ts : fin n → finite_tree}
     {j : fin n} (H : cons ss ≼ ts j) :
   cons ss ≼ cons ts :=
-begin cases m, apply node_embeds, cases n, apply absurd H _, apply not_embeds_empty, apply or.inl (exists.intro j H) end
+begin 
+cases m, 
+apply node_embeds, cases n,
+exact fin_zero_absurd j,
+apply or.inl (exists.intro j H) 
+end
 
-lemma foo {n : ℕ} {f : fin (succ n) → fin 0}  {ss : fin (succ n) → finite_tree} {ts : fin 0 → finite_tree} :
-¬ ∀ a, ss a ≼ ts (f a) := λ h, have ss 0 ≼ ts (f 0), from h 0,
-absurd this (by apply not_embeds_empty)
+-- theorem not_embeds_empty {ts : fin 0 → finite_tree} (i : fin 0) (t : finite_tree) : ¬ t ≼ ts i :=
+-- λ h, have i.val < 0, from i.is_lt, absurd this (not_lt_zero _)
+
+
+-- lemma foo {n : ℕ} {f : fin (succ n) → fin 0}  {ss : fin (succ n) → finite_tree} {ts : fin 0 → finite_tree} :
+-- ¬ ∀ a, ss a ≼ ts (f a) :=  fin_zero_absurd (f 0)
 
 theorem cons_embeds_cons_right {m n : ℕ} {ss : fin m → finite_tree} {ts : fin n → finite_tree}
     {f : fin m → fin n} (injf : injective f) (Hf : ∀ i, ss i ≼ ts (f i)) :
   cons ss ≼ cons ts :=
 begin cases m, apply node_embeds, cases n, 
-apply absurd Hf _, apply foo,
+exact fin_zero_absurd (f 0),
 apply or.inr (exists.intro f (and.intro injf Hf))
 end
 
-theorem cons_embeds_cons_dest {m n : ℕ} {ss : fin m → finite_tree} {ts : fin n → finite_tree}
-    (H : cons ss ≼ cons ts) :
-  (∃ j, cons ss ≼ ts j) ∨ (∃ f, injective f ∧ ∀ i, ss i ≼ ts (f i)) :=
-sorry
--- begin cases m, apply or.inl, end
+-- theorem cons_embeds_cons_dest {m n : ℕ} {ss : fin m → finite_tree} {ts : fin n → finite_tree}
+--     (H : cons ss ≼ cons ts) :
+--   (∃ j, cons ss ≼ ts j) ∨ (∃ f, injective f ∧ ∀ i, ss i ≼ ts (f i)) :=
+-- H
 
 theorem embeds_refl (t : finite_tree) : t ≼ t :=
 begin 
 induction t with n a ih, 
-cases n, trivial, apply cons_embeds_cons_right, 
+cases n, apply node_embeds,
+apply cons_embeds_cons_right, 
 apply injective_id, exact ih 
 end
 
-private def embeds_trans_aux : ∀ {u s t}, t ≼ u → s ≼ t → s ≼ u :=
-λ u s t,finite_tree.rec_on s 
-(λ sl ss ihs, 
-nat.rec_on sl _ _) 
+theorem embeds_trans_aux : ∀ {u s t}, t ≼ u → s ≼ t → s ≼ u :=
+begin
+  intro u,
+  induction u with ul us ihu,
+    intros s t, cases s with sl ss,
+    cases t with tl ts,
+  intro H₁, dsimp [embeds] at H₁, cases H₁ with H₁₁ H₁₂,
+  cases H₁₁ with i H₁₁, intro H₂,
+    apply cons_embeds_cons_left (ihu _ H₁₁ H₂),
+    cases H₁₂ with f Hf, cases Hf with injf Hf,
+  intro H₂, dsimp [embeds] at H₂, cases H₂ with H₂₁ H₂₂,
+    cases H₂₁ with j H₂₁,
+    apply cons_embeds_cons_left (ihu _ (Hf j) H₂₁),
+    cases H₂₂ with g Hg, cases Hg with injg Hg,
+    apply cons_embeds_cons_right,
+    apply injective_comp injf injg,
+    intro i, apply ihu _ (Hf (g i)) (Hg i)
+end
 
--- begin
--- intros u s t,
--- induction s with sl ss ihs,
--- cases sl,
--- {intros,apply node_embeds},
--- {induction t with tl ts iht,
---   cases tl,
---     {intros ht1 ht2, apply absurd ht2, apply not_cons_embeds_node},
---   induction u with ul us ihu,
---     cases ul,
---       intros hu1 hu2, apply absurd hu1, apply not_cons_embeds_node,
---     intros h1 h2,
---     apply cons_embeds_cons_right,-- or.,
---   -- induction h1,
--- },
--- --intros s t, --cases s with n ss,
--- end
-
--- private proposition embeds_trans_aux : ∀ {u s t}, t ≼ u → s ≼ t → s ≼ u :=
--- begin
---   intro u,
---   induction u with l us ihu,
---     intro s t, cases s with n ss,
---       intros, apply node_embeds,
---     cases t, repeat (intros; contradiction),
---   intro s t,
---     cases s with n ss,
---       intros, apply node_embeds,
---     cases t with m ts,
---       intros, contradiction,
---   intro H₁, cases (cons_embeds_cons_dest H₁) with H₁₁ H₁₂,
---     cases H₁₁ with i H₁₁, intro H₂,
---     have cons ss ≼ us i, from ihu _ H₁₁ H₂,
---     apply cons_embeds_cons_left this,
---   cases H₁₂ with f Hf, cases Hf with injf Hf,
---   intro H₂, cases (cons_embeds_cons_dest H₂) with H₂₁ H₂₂,
---     cases H₂₁ with j H₂₁,
---     have cons ss ≼ us (f j), from ihu _ (Hf j) H₂₁,
---     apply cons_embeds_cons_left this,
---   cases H₂₂ with g Hg, cases Hg with injg Hg,
---   apply cons_embeds_cons_right,
---   apply injective_compose injf injg,
---   intro i, apply ihu _ (Hf (g i)) (Hg i)
--- end
-
--- proposition embeds_trans {s t u : finite_tree} (H₁ : s ≼ t) (H₂ : t ≼ u) : s ≼ u :=
--- embeds_trans_aux H₂ H₁
+theorem embeds_trans {s t u : finite_tree} (H₁ : s ≼ t) (H₂ : t ≼ u) : s ≼ u :=
+embeds_trans_aux H₂ H₁
 
 -- proposition cons_embeds_iff {m : ℕ} (ss : fin m → finite_tree) (t : finite_tree) :
 --   cons ss ≼ t ↔ ∃ n (ts : fin n → finite_tree), t = cons ts ∧
